Demo.lean
@@ -1,0 +1,37 @@
+import Strata.Languages.Boogie.ToVelvet
+
+open PartialCorrectness DemonicChoice Lean.Elab.Term.DoNames
+
+set_option auto.smt.trust true
+set_option auto.smt true
+set_option auto.smt.timeout 4
+set_option auto.smt.solver.name "cvc5"
+
+#strataVelvet
+program Boogie;
+
+procedure loopSimple (n: int) returns (r: int)
+spec {
+  requires (n >= 0);
+}
+{
+  var sum : int := 0;
+  var i : int := 0;
+  while (i < n)
+    invariant (i <= n && ((i * (i-1)) div 2 == sum));
+  {
+    sum := sum + i;
+    i := i + 1;
+  }
+  r := sum;
+};
+
+#end
+
+#check Boogie.loopSimple
+#print Boogie.loopSimple
+
+prove_correct Boogie.loopSimple by
+  dsimp [Boogie.loopSimple]
+  loom_solve
+  grind
