Strata/Languages/Boogie/ToVelvet.lean
@@ -1,0 +1,245 @@
+import StrataVerify
+import Strata.DL.Imperative.Stmt
+
+import CaseStudies.Velvet.Syntax
+
+namespace Elab
+
+open Lean Elab Command Term
+open Strata HasInputContext
+open Lean.Parser.Category
+
+structure State where
+  vars : List Boogie.BoogieIdent := []
+
+abbrev TranslateTermM := StateT State TermElabM
+
+def containsVar (id : Boogie.BoogieIdent) : TranslateTermM Bool := do
+  let state ← get
+  return id ∈ state.vars
+
+def toVelvetMonoType (ty : Lambda.LMonoTy) : TranslateTermM (TSyntax `term) := do
+  match ty with
+  | .int  => `($(mkIdent ``Int))
+  | .bool => `($(mkIdent ``Bool))
+  | _ => throwError "Unsupported type {ty}"
+
+def toVelvetType (ty : Boogie.Expression.Ty) : TranslateTermM (TSyntax `term) := do
+  match ty with
+  | .forAll [] mt => toVelvetMonoType mt
+  | _             => throwError "Unsupported type {ty}"
+
+def toVelvetExpr (t : Boogie.Expression.Expr) : TranslateTermM (TSyntax `term) := do
+  match t with
+  | .const c (.some ty) =>
+    match ty with
+    | .int =>
+      let .some c := c.toNat? | throwError "Expected '{c}' to be a natural number"
+      `(term| $(Syntax.mkNatLit c))
+    | .bool => if c == "true" then `($(mkIdent ``true)) else `($(mkIdent ``false))
+    | _ => throwError "Unsupported constant type"
+  | .fvar id ty =>
+    if ← containsVar id then
+      `($(mkIdent id.snd.toName))
+    else if let .some ty := ty then
+      let t ← toVelvetMonoType ty
+      `(@$(mkIdent ``Classical.choice) $t $(mkIdent ``inferInstance))
+    else
+      throwError "Unsupported fvar {t}"
+  | .ite c t e =>
+    let c ← toVelvetExpr c
+    let t ← toVelvetExpr t
+    let e ← toVelvetExpr e
+    `(@$(mkIdent ``ite) $c $t $e)
+  | .app (.app (.op "Bool.And" _) e₁) e₂ =>
+    let e₁ ← toVelvetExpr e₁
+    let e₂ ← toVelvetExpr e₂
+    `($e₁ ∧ $e₂)
+  | .app (.app (.op "Int.Add" _) e₁) e₂ =>
+    let e₁ ← toVelvetExpr e₁
+    let e₂ ← toVelvetExpr e₂
+    `($e₁ + $e₂)
+  | .app (.app (.op "Int.Sub" _) e₁) e₂ =>
+    let e₁ ← toVelvetExpr e₁
+    let e₂ ← toVelvetExpr e₂
+    `($e₁ - $e₂)
+  | .app (.app (.op "Int.Mul" _) e₁) e₂ =>
+    let e₁ ← toVelvetExpr e₁
+    let e₂ ← toVelvetExpr e₂
+    `($e₁ * $e₂)
+  | .app (.app (.op "Int.Div" _) e₁) e₂ =>
+    let e₁ ← toVelvetExpr e₁
+    let e₂ ← toVelvetExpr e₂
+    `($e₁ / $e₂)
+  | .app (.app (.op "Int.Lt" _) e₁) e₂ =>
+    let e₁ ← toVelvetExpr e₁
+    let e₂ ← toVelvetExpr e₂
+    `($e₁ < $e₂)
+  | .app (.app (.op "Int.Le" _) e₁) e₂ =>
+    let e₁ ← toVelvetExpr e₁
+    let e₂ ← toVelvetExpr e₂
+    `($e₁ ≤ $e₂)
+  | .app (.app (.op "Int.Ge" _) e₁) e₂ =>
+    let e₁ ← toVelvetExpr e₁
+    let e₂ ← toVelvetExpr e₂
+    `($e₁ ≥ $e₂)
+  | .app (.app (.op "Int.Gt" _) e₁) e₂ =>
+    let e₁ ← toVelvetExpr e₁
+    let e₂ ← toVelvetExpr e₂
+    `($e₁ > $e₂)
+  | .eq e₁ e₂ =>
+    let e₁ ← toVelvetExpr e₁
+    let e₂ ← toVelvetExpr e₂
+    `($e₁ = $e₂)
+  | _ => throwError "Unsupported expr {t}"
+
+open Lambda.LExpr.Syntax
+open Lambda.LExpr.SyntaxMono
+
+abbrev VelvetHeader := TSyntax `ident × TSyntaxArray `leafny_binder × TSyntax `ident × TSyntax `term
+
+def toVelvetProcedureHeader (h : Boogie.Procedure.Header) : TranslateTermM VelvetHeader := do
+  let name ← `(ident| $(mkIdent (`Boogie ++ h.name.snd.toName)))
+  let params : Array (TSyntax `leafny_binder) ← h.inputs.toArray.mapM toVelvetParam
+  let [(id, ty)] := h.outputs | throwError "Expected exactly one output"
+  let outName ← `(ident| $(mkIdent id.snd.toName))
+  let outType ← toVelvetMonoType ty
+  return (name, params, outName, outType)
+where
+  toVelvetParam (id : Boogie.BoogieIdent × Lambda.LMonoTy) : TranslateTermM (TSyntax `leafny_binder) := do
+    let (name, ty) := id
+    modify fun s => { s with vars := name :: s.vars }
+    let name ← `(ident| $(mkIdent name.snd.toName))
+    let type ← toVelvetMonoType ty
+    `(leafny_binder| (mut $name : $type))
+
+abbrev VelvetSpec := TSyntaxArray `term × TSyntaxArray `term
+
+def toVelvetSpec (s : Boogie.Procedure.Spec) : TranslateTermM VelvetSpec := do
+  let reqs ← s.preconditions.toArray.mapM toVelvetCheck
+  let enss ← s.postconditions.toArray.mapM toVelvetCheck
+  return (reqs, enss)
+where
+  toVelvetCheck (c : Boogie.BoogieLabel × Boogie.Procedure.Check) :=
+    toVelvetExpr c.snd.expr
+
+mutual
+
+def toVelvetStatement (out : Boogie.BoogieIdent) (s : Boogie.Statement) : TranslateTermM (TSyntax `doElem) := do
+  match s with
+  | .init id ty v =>
+    let name ← `(ident| $(mkIdent id.snd.toName))
+    modify fun s => { s with vars := id :: s.vars }
+    let type ← toVelvetType ty
+    let e ← if let .fvar id _ := v then
+              if ← containsVar id then
+                `($(mkIdent id.snd.toName))
+              else
+                -- Case: `var x : T := init_*`
+                -- TODO: `init_*` should probably be declared as a global variable
+                `(@Classical.choice $type inferInstance)
+            else
+              toVelvetExpr v
+    `(doElem| let mut $name : $type := $e)
+  | .set id v =>
+    let e ← toVelvetExpr v
+    if id = out then
+      `(doElem| return $e)
+    else
+      let name ← `(ident| $(mkIdent id.snd.toName))
+      if ← containsVar id then
+        let reassign ← `(Lean.Parser.Term.doReassign| $name := $e)
+        return ⟨reassign⟩
+      else
+        throwError "Unknown variable {id}"
+  | .ite c t e md =>
+    have : sizeOf t.ss < sizeOf (Imperative.Stmt.ite c t e md) := by simp +arith [sizeOf]
+    have : sizeOf e.ss < sizeOf (Imperative.Stmt.ite c t e md) := by simp [sizeOf]
+    let c ← toVelvetExpr c
+    let t ← toVelvetBlock out t.ss
+    let e ← toVelvetBlock out e.ss
+    `(doElem| if $c then $[$t:doElem]* else $[$e:doElem]*)
+  | .loop c m i b md =>
+    have : sizeOf b.ss < sizeOf (Imperative.Stmt.loop c m i b md) := by simp [sizeOf]
+    let c ← toVelvetExpr c
+    let m ← m.mapM toVelvetExpr
+    let i ← i.toArray.mapM toVelvetExpr
+    let b ← toVelvetBlock out b.ss
+    `(doElem| while $c
+      $[invariant $i]*
+      $[decreasing $m]?
+      do
+        $[$b:doElem]*)
+  | _ => throwError s!"Unsupported statement"
+
+def toVelvetBlock (out : Boogie.BoogieIdent) (ss : Boogie.Statements) : TranslateTermM (TSyntaxArray `doElem) := do
+  let ss ← ss.attach.mapM fun ⟨s, h⟩ =>
+    have : sizeOf s < sizeOf ss := by simp [Imperative.Stmts.sizeOf_lt_of_mem h]
+    toVelvetStatement out s
+  return ss.toArray
+
+end
+
+def toVelvetBody (out : Boogie.BoogieIdent) (ss : Boogie.Statements) : TranslateTermM doSeq := do
+  let ss ← ss.toArray.mapM (toVelvetStatement out)
+  `(doSeq| $[$ss:doElem]*)
+
+abbrev TranslateCmdM := StateT State CommandElabM
+
+def liftTranslateTermM {α} (x : TranslateTermM α) : TranslateCmdM α := do
+  let s ← get
+  let (a, s') ← liftTermElabM (StateT.run x s)
+  set s'
+  return a
+
+def toVelvetProcedure (p : Boogie.Procedure) : TranslateCmdM (TSyntax `command) := do
+  let state ← get
+  let [(out, _)] := p.header.outputs | throwError "Expected exactly one output"
+  let (name, params, outName, outType) ← liftTranslateTermM (toVelvetProcedureHeader p.header)
+  let (reqs, enss) ← liftTranslateTermM (toVelvetSpec p.spec)
+  let body ← liftTranslateTermM (toVelvetBody out p.body)
+  set { state with vars := p.header.name :: state.vars }
+  `(method $name $params* return ($outName : $outType)
+    $[require $reqs]*
+    $[ensures $enss]*
+    do
+      $body)
+
+def toVelvetDecl (d : Boogie.Decl) : TranslateCmdM (TSyntax `command) := do
+  match d with
+  | .proc d _ => toVelvetProcedure d
+  | _ => throwError s!"Unexpected declaration: {d.name}"
+
+def toVelvetBoogie (p : Boogie.Program) : TranslateCmdM (TSyntaxArray `command) := do
+  p.decls.toArray.mapM toVelvetDecl
+
+def toVelvet (program : Strata.Program) : CommandElabM Unit := do
+  let cmds ← match program.dialect with
+    | "Boogie" =>
+      let (program, errors) := Strata.TransM.run (Strata.translateProgram program)
+      let #[] := errors | throwError s!"DDM Transform Error: {errors}"
+      logInfo f!"AST: {program}"
+      (toVelvetBoogie program).run' {}
+    | _ => throwError s!"Unknown dialect: {program.dialect}"
+  cmds.forM (logInfo m!"{·}")
+  cmds.forM elabCommand
+
+declare_tagged_region command strataVelvetProgram "#strataVelvet" "#end"
+
+@[command_elab strataVelvetProgram]
+def strataVelvetProgramImpl : CommandElab := fun (stx : Syntax) => do
+  let .atom i v := stx[1]
+        | throwError s!"Bad {stx[1]}"
+  let .original _ p _ e := i
+        | throwError s!"Expected input context"
+  let inputCtx ← getInputContext
+  let loader := (dialectExt.getState (←Lean.getEnv)).loaded
+  let leanEnv ← Lean.mkEmptyEnvironment 0
+  match Elab.elabProgram loader leanEnv inputCtx p e with
+  | .ok pgm =>
+    toVelvet pgm
+  | .error errors =>
+    for (stx, e) in errors do
+      logMessage e
+
+end Elab
